1.$a_j^{(l)} = f\left(\sum_k w_{jk}^{(l)} a_k^{(l-1)} + b_j^{(l)}\right)$
2. $$J = \frac{1}{2n}\sum_{i=1}^n (a_i^{(L)} - y_i)^2$$

3. $$a_j^{(1)} = x_j$$

4. $$a_j^{(l)} = f(\sum_k w_{jk}^{(l)} a_k^{(l-1)} + b_j^{(l)})\ \ \ \ \ \ \ \(l = 2,...,L)\ \ \ \ \ \ \ \ (2)$$
5. $$J = \frac{1}{2n}\sum_{i=1}^n (a_i^{(L)} - y_i)^2\ \ \ \ \ \ \ \ (2)$$

$$a_j^{(1)} = x_j$$

$$a_j^(l)\ =\ f(\sum_k\ w_{j}^{l） a_k^(l-1) + b_j^(l))$$                   (l = 2,…,L)

$$J\ =\ \frac{1}{2n}\sum_i\ (a_i^{(L）} - y_i)^2$$
